@prefix : <http://cor.esipfed.org/ont/earthcube/srt#> .
@prefix dc: <http://purl.org/dc/elements/1.1/> .
@prefix owl: <http://www.w3.org/2002/07/owl#> .
@prefix rdf: <http://www.w3.org/1999/02/22-rdf-syntax-ns#> .
@prefix xml: <http://www.w3.org/XML/1998/namespace> .
@prefix xsd: <http://www.w3.org/2001/XMLSchema#> .
@prefix rdfs: <http://www.w3.org/2000/01/rdf-schema#> .
@prefix oboInOwl: <http://www.geneontology.org/formats/oboInOwl#> .
@base <http://cor.esipfed.org/ont/earthcube/srt> .

<http://cor.esipfed.org/ont/earthcube/srt> rdf:type owl:Ontology ;
                                            <http://purl.org/dc/elements/1.1/description> "The Semantic Resource Types Vocabulary was created for NSF's EarthCube Program's Resource Repository.  At this point it merely lists the types of semantic resources in the repository.  Primary use case - give me a list of the ontologies in use within EarthCube projects."@en ;
                                            <http://purl.org/dc/elements/1.1/title> "Semantic Resource Types Vocabulary"@en ;
                                            <http://purl.org/dc/terms/bibliographicCitation> "Duerr, R., 2019, \"Semantic Resource Types Vocabulary\", ESIP Community Ontology Repository, Version 1.0.0, available at: http://cor.esipfed.org/ont/earthcube/srt"@en ;
                                            <http://purl.org/dc/terms/license> <https://creativecommons.org/share-your-work/public-domain/cc0/> ,
                                                                               "Ruth Duerr"@en ;
                                            owl:versionInfo "1.0.0"@en .

#################################################################
#    Annotation properties
#################################################################

###  http://purl.obolibrary.org/obo/IAO_0000115
<http://purl.obolibrary.org/obo/IAO_0000115> rdf:type owl:AnnotationProperty ;
                                             rdfs:label "definition" .


###  http://purl.obolibrary.org/obo/IAO_0000119
<http://purl.obolibrary.org/obo/IAO_0000119> rdf:type owl:AnnotationProperty ;
                                             rdfs:label "definition source" .


###  http://purl.org/dc/elements/1.1/creator
<http://purl.org/dc/elements/1.1/creator> rdf:type owl:AnnotationProperty .


###  http://purl.org/dc/elements/1.1/description
<http://purl.org/dc/elements/1.1/description> rdf:type owl:AnnotationProperty .


###  http://purl.org/dc/elements/1.1/title
<http://purl.org/dc/elements/1.1/title> rdf:type owl:AnnotationProperty .


###  http://purl.org/dc/terms/bibliographicCitation
<http://purl.org/dc/terms/bibliographicCitation> rdf:type owl:AnnotationProperty .


###  http://purl.org/dc/terms/license
<http://purl.org/dc/terms/license> rdf:type owl:AnnotationProperty .


###  http://www.geneontology.org/formats/oboInOwl#created_by
<http://www.geneontology.org/formats/oboInOwl#created_by> rdf:type owl:AnnotationProperty .


###  http://www.geneontology.org/formats/oboInOwl#creation_date
<http://www.geneontology.org/formats/oboInOwl#creation_date> rdf:type owl:AnnotationProperty .


###  http://www.geneontology.org/formats/oboInOwl#hasDbXref
<http://www.geneontology.org/formats/oboInOwl#hasDbXref> rdf:type owl:AnnotationProperty .


###  http://www.geneontology.org/formats/oboInOwl#hasExactSynonym
<http://www.geneontology.org/formats/oboInOwl#hasExactSynonym> rdf:type owl:AnnotationProperty .


###  http://www.geneontology.org/formats/oboInOwl#hasRelatedSynonym
<http://www.geneontology.org/formats/oboInOwl#hasRelatedSynonym> rdf:type owl:AnnotationProperty .


###  http://www.geneontology.org/formats/oboInOwl#hasURI
<http://www.geneontology.org/formats/oboInOwl#hasURI> rdf:type owl:AnnotationProperty .


#################################################################
#    Classes
#################################################################

###  http://cor.esipfed.org/ont/earthcube/srt_0000001
<http://cor.esipfed.org/ont/earthcube/srt_0000001> rdf:type owl:Class ;
                                                   rdfs:subClassOf <http://cor.esipfed.org/ont/earthcube/srt_0000009> ;
                                                   <http://purl.obolibrary.org/obo/IAO_0000115> "A semantic resource that only consists of a set of terms and their definitions, possibly including synonyms."@en ;
                                                   <http://www.geneontology.org/formats/oboInOwl#created_by> <http://orcid.org/0000-0003-4808-4736> ;
                                                   <http://www.geneontology.org/formats/oboInOwl#creation_date> "2019-10-22T04:37:33Z"^^xsd:dateTime ;
                                                   rdfs:comment "Examples: NSIDC's Cryosphere Glossary https://nsidc.org/cryosphere/glossary"@en ;
                                                   rdfs:label "Glossary"@en .


###  http://cor.esipfed.org/ont/earthcube/srt_0000002
<http://cor.esipfed.org/ont/earthcube/srt_0000002> rdf:type owl:Class ;
                                                   rdfs:subClassOf <http://cor.esipfed.org/ont/earthcube/srt_0000009> ;
                                                   <http://purl.obolibrary.org/obo/IAO_0000115> "A semantic resource consisting of a structured controlled vocabulary where there is information about each term and its hierarchical, associative, or equivalence relationships to other terms in the thesaurus."@en ;
                                                   <http://www.geneontology.org/formats/oboInOwl#created_by> <http://orcid.org/0000-0003-4808-4736> ;
                                                   <http://www.geneontology.org/formats/oboInOwl#creation_date> "2019-10-22T04:40:05Z"^^xsd:dateTime ;
                                                   rdfs:label "Thesaurus"@en .


###  http://cor.esipfed.org/ont/earthcube/srt_0000003
<http://cor.esipfed.org/ont/earthcube/srt_0000003> rdf:type owl:Class ;
                                                   rdfs:subClassOf <http://cor.esipfed.org/ont/earthcube/srt_0000009> ;
                                                   <http://purl.obolibrary.org/obo/IAO_0000115> "A semantic resource containing a set of concepts with attributes and relationships between the concepts which together define a domain of knowledge, expressed in machine-readable format."@en ;
                                                   <http://www.geneontology.org/formats/oboInOwl#created_by> <http://orcid.org/0000-0003-4808-4736> ;
                                                   <http://www.geneontology.org/formats/oboInOwl#creation_date> "2019-10-22T04:41:32Z"^^xsd:dateTime ;
                                                   rdfs:label "Ontology"@en .


###  http://cor.esipfed.org/ont/earthcube/srt_0000004
<http://cor.esipfed.org/ont/earthcube/srt_0000004> rdf:type owl:Class ;
                                                   rdfs:subClassOf <http://cor.esipfed.org/ont/earthcube/srt_0000009> ;
                                                   <http://purl.obolibrary.org/obo/IAO_0000115> "A semantic resource consisting of a list of terms controlled by some authority, generally intended to populate pick lists in user interfaces."@en ;
                                                   <http://www.geneontology.org/formats/oboInOwl#created_by> <http://orcid.org/0000-0003-4808-4736> ;
                                                   <http://www.geneontology.org/formats/oboInOwl#creation_date> "2019-10-22T04:42:17Z"^^xsd:dateTime ;
                                                   rdfs:comment "Assumption is that users will all understand the terms without any additional guidance."@en ;
                                                   rdfs:label "Controlled Vocabulary"@en .


###  http://cor.esipfed.org/ont/earthcube/srt_0000005
<http://cor.esipfed.org/ont/earthcube/srt_0000005> rdf:type owl:Class ;
                                                   rdfs:subClassOf <http://cor.esipfed.org/ont/earthcube/srt_0000009> ;
                                                   <http://purl.obolibrary.org/obo/IAO_0000115> "A semantic resource made up of hierarchies of terms organized as tree structures without significant relationships to concepts in other trees."@en ;
                                                   <http://www.geneontology.org/formats/oboInOwl#created_by> <http://orcid.org/0000-0003-4808-4736> ;
                                                   <http://www.geneontology.org/formats/oboInOwl#creation_date> "2019-10-22T04:43:21Z"^^xsd:dateTime ;
                                                   rdfs:comment "Example: domain, kingdom, phylum or division, class, genus, species is the taxonomic heirarchy in Biology."@en ;
                                                   rdfs:label "Taxonomy"@en .


###  http://cor.esipfed.org/ont/earthcube/srt_0000006
<http://cor.esipfed.org/ont/earthcube/srt_0000006> rdf:type owl:Class ;
                                                   rdfs:subClassOf <http://cor.esipfed.org/ont/earthcube/srt_0000009> ;
                                                   <http://purl.obolibrary.org/obo/IAO_0000115> "A semantic resource consisting of an information model represented with artifacts such as diagrams (e.g. UML, concept maps) and associated text, not formalized as an ontology."@en ;
                                                   <http://www.geneontology.org/formats/oboInOwl#created_by> <http://orcid.org/0000-0003-4808-4736> ;
                                                   <http://www.geneontology.org/formats/oboInOwl#creation_date> "2019-10-22T04:49:05Z"^^xsd:dateTime ;
                                                   rdfs:label "Conceptual Model"@en .


###  http://cor.esipfed.org/ont/earthcube/srt_0000007
<http://cor.esipfed.org/ont/earthcube/srt_0000007> rdf:type owl:Class ;
                                                   rdfs:subClassOf <http://cor.esipfed.org/ont/earthcube/srt_0000009> ;
                                                   <http://purl.obolibrary.org/obo/IAO_0000115> "A semantic resource containing a representation of a knowledge domain that defines rdf classes and attributes, along with domain and range constraints for some attributes."@en ;
                                                   <http://www.geneontology.org/formats/oboInOwl#created_by> <http://orcid.org/0000-0003-4808-4736> ;
                                                   <http://www.geneontology.org/formats/oboInOwl#creation_date> "2019-10-22T04:50:36Z"^^xsd:dateTime ;
                                                   <http://www.geneontology.org/formats/oboInOwl#hasExactSynonym> "Resource Description Framework vocabulary"@en ;
                                                   rdfs:comment "Distinguish from more formal ontologies by absence of general class relationships, and restrictions offered by representations like OWL."@en ;
                                                   rdfs:label "RDF vocabulary"@en .


###  http://cor.esipfed.org/ont/earthcube/srt_0000008
<http://cor.esipfed.org/ont/earthcube/srt_0000008> rdf:type owl:Class ;
                                                   rdfs:subClassOf <http://cor.esipfed.org/ont/earthcube/srt_0000009> ;
                                                   <http://purl.obolibrary.org/obo/IAO_0000115> "A semantic resource comprised of a collection of concepts with identifiers, preferred labels, and definitions; including broader, narrower, related and transitive relationships, labels in alternate languages, and other annotation properties."@en ;
                                                   <http://www.geneontology.org/formats/oboInOwl#created_by> <http://orcid.org/0000-0003-4808-4736> ;
                                                   <http://www.geneontology.org/formats/oboInOwl#creation_date> "2019-10-22T04:52:45Z"^^xsd:dateTime ;
                                                   rdfs:comment "Encoded using SKOS rdf vocabulary."@en ,
                                                                "Glossary, Taxonomy,  and Thesaurus might be represented using SKOS vocabulary, but each lack one or more of the semantic enhancments offered by SKOS."@en ;
                                                   rdfs:label "SKOS vocabulary"@en .


###  http://cor.esipfed.org/ont/earthcube/srt_0000009
<http://cor.esipfed.org/ont/earthcube/srt_0000009> rdf:type owl:Class ;
                                                   <http://purl.obolibrary.org/obo/IAO_0000115> "A categorization of the kind of semantic resource a given resource is."@en ;
                                                   <http://www.geneontology.org/formats/oboInOwl#created_by> <http://orcid.org/0000-0003-4808-4736> ;
                                                   <http://www.geneontology.org/formats/oboInOwl#creation_date> "2019-10-22T04:55:49Z"^^xsd:dateTime ;
                                                   rdfs:label "Semantic Resource Type"@en .


###  Generated by the OWL API (version 4.5.7.2018-12-02T02:23:35Z) https://github.com/owlcs/owlapi
